ulib/FStar.ModifiesGen.fsti
@@ -899,15 +899,19 @@ val modifies_upd
   (ensures (modifies #_ #c (loc_mreference r) h (HS.upd h r v)))
 
 val modifies_strengthen
-  (#al: aloc_t) (#c: cls al) (l: loc c) (#r0: HS.rid) (#a0: nat) (al0: al r0 a0) (al1: al r0 a0) (h h' : HS.mem)
+  (#al: aloc_t) (#c: cls al) (l: loc c) (#r0: HS.rid) (#a0: nat) (al0: al r0 a0) (h h' : HS.mem)
   (alocs: (
+    (f: ((t: Type) -> (pre: Preorder.preorder t) -> (m: HS.mreference t pre) -> Lemma
+      (requires (HS.frameOf m == r0 /\ HS.as_addr m == a0 /\ HS.contains h m))
+      (ensures (HS.contains h' m))
+    )) ->
     (x: al r0 a0) ->
     Lemma
     (requires (c.aloc_disjoint x al0))
     (ensures (c.aloc_preserved x h h'))
   ))
 : Lemma
-  (requires (modifies (loc_union l (loc_of_aloc al1)) h h'))
+  (requires (modifies (loc_union l (loc_addresses true r0 (Set.singleton a0))) h h'))
   (ensures (modifies (loc_union l (loc_of_aloc al0)) h h'))
 
 (** BEGIN TODO: move to FStar.Monotonic.HyperStack *)
